major cleanup including some improvements from RM

bfn.v
@@ -17,7 +17,7 @@
 *)
 
 Require Import List Arith Omega Wellfounded.
-Require Import utils bt bft.
+Require Import list_utils wf_utils bt bft.
 
 Set Implicit Arguments.
 
@@ -83,12 +83,50 @@ Section bfn.
           2) the result is a breadth first numbering from n  
    *)
 
-  Fixpoint bfn_f n (l : list (bt X)) (D : Acc (fun x y => lsum x < lsum y) l) : { m | l ~lt m /\ is_bfn_from n m }.
+  Definition bfn_f n (l : list (bt X)) : { m | l ~lt m /\ is_bfn_from n m }.
   Proof.
+    double measure induction on n l with (lsum l).
+    intros n l bfn_f.
+
     refine (match l as l' return l = l' -> _ with
       | nil              => fun H => exist _ nil _
       | leaf x :: ll     => fun H => let (mm,Hm) := bfn_f (S n) ll _ in exist _ (leaf n::mm) _
       | node a x b :: ll => fun H => let (mm,Hmm) := bfn_f (S n) (ll++a::b::nil) _ in 
+                                     match list_snoc_match mm _ with
+                                       | existT _ v (existT _ u (exist _ m Hm)) => exist _ (node u n v::m) _
+                                     end
+    end eq_refl).
+    1,2,4,5: cycle 1.
+
+    + subst; simpl; auto.
+    + subst; simpl; rewrite lsum_app; simpl; omega.
+
+    + apply proj1, Forall2_length in Hmm.
+      rewrite <- Hmm, app_length; simpl; omega.
+    + subst; split.
+      * constructor.
+      * red; rewrite bft_f_fix_0; simpl; auto.
+    + destruct Hm as (H1 & H2).
+      subst; split; auto.
+      red in H2 |- *; rewrite bft_f_fix_3.
+      simpl; rewrite <- app_nil_end; auto.
+    + subst; destruct Hmm as (H1 & H2).
+      Forall2 inv H1 as H3.
+      * Forall2 inv H1 as H4.
+        Forall2 inv H1 as H5.
+        split; auto.
+        red in H2 |- *. 
+        rewrite bft_f_fix_3; simpl; auto.
+      * apply Forall2_length in H1. 
+        repeat rewrite app_length in H1; simpl in H1; omega.
+  Defined.
+
+  Fixpoint bfn_f' n (l : list (bt X)) (D : Acc (fun x y => lsum x < lsum y) l) : { m | l ~lt m /\ is_bfn_from n m }.
+  Proof.
+    refine (match l as l' return l = l' -> _ with
+      | nil              => fun H => exist _ nil _
+      | leaf x :: ll     => fun H => let (mm,Hm) := bfn_f' (S n) ll _ in exist _ (leaf n::mm) _
+      | node a x b :: ll => fun H => let (mm,Hmm) := bfn_f' (S n) (ll++a::b::nil) _ in 
                                      match list_snoc_match mm _ with
                                        | existT _ v (existT _ u (exist _ m Hm)) => exist _ (node u n v::m) _
                                      end
@@ -123,14 +161,14 @@ Section bfn.
 
     Let bfn_full (t : bt X) : { t' | t ~t t' /\ is_seq_from 0 (bft_std t') }.
     Proof.
-      refine (match @bfn_f 0 (t::nil) _ with
+      refine (match @bfn_f 0 (t::nil) with
         | exist _ l Hl      => 
         match l as l' return l = l' -> _ with
           | nil   => fun E => _
           | t'::l => fun E => exist _ t' _
         end eq_refl
       end); simpl in *.
-      + apply Acc_measure.
+ (*     + apply Acc_measure. *)
       + exfalso; subst; apply proj1 in Hl; inversion Hl.
       + subst; destruct Hl as (H1 & H2).
         Forall2 inv H1 as H3.
@@ -152,7 +190,7 @@ Section bfn.
 
 End bfn.
 
-Recursive Extraction bfn.
+Recursive Extraction bfn bfn_f'.
 
 Check bfn.
 Check bfn_spec_1.
