sorted.v
@@ -1,0 +1,93 @@
+(**************************************************************)
+(*   Copyright Dominique Larchey-Wendling [*]                 *)
+(*                                                            *)
+(*                             [*] Affiliation LORIA -- CNRS  *)
+(**************************************************************)
+(*      This file is distributed under the terms of the       *)
+(*         CeCILL v2 FREE SOFTWARE LICENSE AGREEMENT          *)
+(**************************************************************)
+
+Require Import List Arith Omega Wellfounded Permutation.
+
+Require Import list_utils php.
+
+Set Implicit Arguments.
+
+Section sorted.
+
+  Variable (X : Type) (R : X -> X -> Prop).
+
+  Inductive sorted : list X -> Prop :=
+    | in_sorted_0 : sorted nil
+    | in_sorted_1 : forall x l, Forall (R x) l -> sorted l -> sorted (x::l).
+
+  Fact sorted_app l m : (forall x y, In x l -> In y m -> R x y) -> sorted l -> sorted m -> sorted (l++m).
+  Proof.
+    intros H H1 Hm; revert H1 H.
+    induction 1 as [ | x l H1 H2 IH2 ]; intros H3; simpl; auto.
+    constructor.
+    + apply Forall_app; auto.
+      apply Forall_forall; intros; apply H3; simpl; auto.
+    + apply IH2; intros; apply H3; simpl; auto.
+  Qed.
+
+  Variable (f : X -> X) (Hf : forall x y, R x y -> R (f x) (f y)).
+
+  Fact sorted_map l : sorted l -> sorted (map f l).
+  Proof.
+    induction 1 as [ | x l H1 H2 IH2 ]; simpl; constructor; auto.
+    apply Forall_forall.
+    rewrite Forall_forall in H1.
+    intros y; rewrite in_map_iff.
+    intros (? & ? & ?); subst; auto.
+  Qed.
+
+End sorted.
+
+Fact sorted_mono X (R S : X -> X -> Prop) l : (forall x y, In x l -> In y l -> R x y -> S x y) -> sorted R l -> sorted S l.
+Proof.
+  intros H1 H2; revert H2 H1.
+  induction 1 as [ | x l H1 H2 IH2 ]; intros H3.
+  + constructor.
+  + constructor.
+    * revert H1; do 2 rewrite Forall_forall.
+      intros H1 y Hy; apply H3; simpl; auto.
+    * apply IH2; intros ? ? ? ?; apply H3; simpl; auto.
+Qed.
+
+Section sorted_no_dup.
+ 
+  Variables (X : Type) (R : X -> X -> Prop) (HR : forall x, ~ R x x).
+
+  Lemma sorted_no_dup l : sorted R l -> ~ list_has_dup l.
+  Proof.
+    induction 1 as [ | x l H1 H2 IH2 ]; intros H.
+    + inversion H.
+    + apply list_hd_cons_inv in H.
+      destruct H as [ H | H ]; try tauto.
+      rewrite Forall_forall in H1; firstorder.
+  Qed.
+
+End sorted_no_dup.
+
+Section sorted_perm.
+
+  Variables (X : Type) (R S : X -> X -> Prop)
+            (HR : forall x, ~ R x x) (HS : forall x, ~ S x x)
+            (l m : list X) (Hl : sorted R l) (Hm : sorted S m) 
+            (Hlm : forall x, In x l <-> In x m).
+
+  Theorem sorted_perm : l ~p m.
+  Proof.
+    destruct (le_lt_dec (length l) (length m)) as [ H | H ].
+    + destruct (@length_le_and_incl_implies_dup_or_perm _ l m) as [ C | C ]; auto.
+      * intro; apply Hlm.
+      * contradict C; revert Hm; apply sorted_no_dup, HS.
+      * apply Permutation_sym; auto.
+    + destruct (@length_le_and_incl_implies_dup_or_perm _ m l) as [ C | C ]; auto.
+      * omega.
+      * intro; apply Hlm.
+      * contradict C; revert Hl; apply sorted_no_dup, HR.
+  Qed.
+
+End sorted_perm.
