wf_utils.v
@@ -1,0 +1,58 @@
+(**************************************************************)
+(*   Copyright Dominique Larchey-Wendling [*]                 *)
+(*                                                            *)
+(*                             [*] Affiliation LORIA -- CNRS  *)
+(**************************************************************)
+(*      This file is distributed under the terms of the       *)
+(*         CeCILL v2 FREE SOFTWARE LICENSE AGREEMENT          *)
+(**************************************************************)
+
+Require Import Arith Omega Wellfounded Extraction.
+
+Set Implicit Arguments.
+
+Section measure_rect.
+
+  Variable (X : Type) (m : X -> nat) (P : X -> Type)
+           (HP : forall x, (forall y, m y < m x -> P y) -> P x).
+
+  Let R x y := m x < m y.
+
+  Fact Acc_measure : well_founded R.
+  Proof. unfold R; apply wf_inverse_image, lt_wf. Qed.
+
+  Theorem measure_rect x : P x.
+  Proof.
+    cut (Acc R x).
+    + revert x.
+      exact (fix loop x Hx { struct Hx } := @HP x (fun y Hy => loop y (Acc_inv Hx Hy))).
+    + apply Acc_measure.
+  Qed.
+
+End measure_rect.
+
+Section measure_double_rect.
+
+  Variable (X Y : Type) (m : X -> Y -> nat) (P : X -> Y -> Type)
+           (HP : forall x y, (forall x' y', m x' y' < m x y -> P x' y') -> P x y).
+
+  Let R c d := m (fst c) (snd c) < m (fst d) (snd d).
+
+  Theorem measure_double_rect x y : P x y.
+  Proof.
+    cut (Acc R (x,y)).
+    + revert x y.
+      refine (fix loop x y H { struct H } := @HP x y (fun x' y' H' => loop x' y' (Acc_inv H _))).
+      apply H'.
+    + unfold R; apply wf_inverse_image, lt_wf.
+  Qed.
+
+End measure_double_rect.
+
+Tactic Notation "measure" "induction" "on" hyp(x) "with" uconstr(f) :=
+  pattern x; revert x; apply measure_rect with (m := fun x => f).
+
+Tactic Notation "double" "measure" "induction" "on" hyp(x) hyp(y) "with" uconstr(f) :=
+  pattern x, y; revert x y; apply measure_double_rect with (m := fun x y => f).
+
+Extraction Inline measure_rect measure_double_rect.
